Move def of roll_back to be directly usable from bootstrap trans

compiler/repl/repl_check_and_tweakScript.sml
@@ -75,4 +75,23 @@ Theorem safe_exp_pmatch = safe_exp_pmatch_lemma
                        candle_kernel_valsTheory.kernel_ffi_def,
                        IN_UNION,IN_INSERT,NOT_IN_EMPTY,GSYM CONJ_ASSOC]
 
+(* used in repl_types and repl-function in compiler64Prog *)
+
+Definition roll_back_def:
+  roll_back (old_ienv, old_next_id) (new_ienv, new_next_id) =
+    (old_ienv, new_next_id)
+End
+
+Theorem FST_roll_back[simp]:
+  FST (roll_back x y) = FST x
+Proof
+  Cases_on`x` \\ Cases_on`y` \\ rw[roll_back_def]
+QED
+
+Theorem SND_roll_back[simp]:
+  SND (roll_back x y) = SND y
+Proof
+  Cases_on`x` \\ Cases_on`y` \\ rw[roll_back_def]
+QED
+
 val _ = export_theory();
