compiler/repl/repl_typesScript.sml
@@ -26,23 +26,6 @@ Definition check_ref_types_def:
     nsLookup env.v name = SOME (Loc loc)
 End
 
-Definition roll_back_def:
-  roll_back (old_ienv, old_next_id) (new_ienv, new_next_id) =
-    (old_ienv, new_next_id)
-End
-
-Theorem FST_roll_back[simp]:
-  FST (roll_back x y) = FST x
-Proof
-  Cases_on`x` \\ Cases_on`y` \\ rw[roll_back_def]
-QED
-
-Theorem SND_roll_back[simp]:
-  SND (roll_back x y) = SND y
-Proof
-  Cases_on`x` \\ Cases_on`y` \\ rw[roll_back_def]
-QED
-
 Inductive repl_types:
 [repl_types_init:]
   (∀ffi rs decs types (s:'ffi semanticPrimitives$state) env ck b.
